\documentclass{article}
\usepackage{enumerate}
\usepackage{amsmath}
\usepackage{amssymb}
\usepackage{graphicx}
\usepackage{subfigure}
\usepackage{geometry}
\usepackage{caption}
\usepackage{indentfirst}
\geometry{left=3.0cm,right=3.0cm,top=3.0cm,bottom=4.0cm}
\usepackage{ctex}
\renewcommand\thesection{Ex \arabic{section}.}
\DeclareMathOperator*{\suplim}{\overline{\lim}}
\DeclareMathOperator*{\inflim}{\underline{\lim}}

\title{MA426 DIFFERENTIAL GEOMETRY HOMEWORK 1}
\author{刘逸灏 515370910207}
\date{\today}

\begin{document}
\maketitle

\section{}
Suppose the angular velocity of the disk is $\omega$, let the straight line be the $x$ axis and suppose that the center of disk is $(0,a)$ and M is at $(a,a)$ in the initial state. Then
$$\alpha(t)=(a\omega t+a\cos\omega t,a+a\sin\omega t)$$

\section{}
$$x=e^t,y=e^{-t},z=t\sqrt{2}$$
\begin{align*}
\kappa(t)&=\frac{\sqrt{(z''y'-y''z')^2+(x''z'-z''x')^2+(y''x'-x''y')^2}}{\sqrt{x'^2+y'^2+z'^2}^3}\\
&=\frac{\sqrt{2e^{-2t}+2e^{2t}+4}}{\sqrt{e^{2t}+e^{-2t}+2}^3}
=\frac{\sqrt{2}}{(e^t+e^{-t})^2}
\end{align*}
\begin{align*}
\tau(t)&=-\frac{x'''(z''y'-y''z')+y'''(x''z'-z''x')+z'''(y''x'-x''y')}{(z''y'-y''z')^2+(x''z'-z''x')^2+(y''x'-x''y')^2}\\
&=-\frac{-\sqrt{2}-\sqrt{2}}{2e^{-2t}+2e^{2t}+4}
=\frac{\sqrt{2}}{(e^t+e^{-t})^2}
\end{align*}

$$x=\cos^3t,y=\sin^3t,z=\cos2t$$
\begin{align*}
\kappa(t)&=\frac{\sqrt{(z''y'-y''z')^2+(x''z'-z''x')^2+(y''x'-x''y')^2}}{\sqrt{x'^2+y'^2+z'^2}^3}\\
&=\frac{15\sin^2t(1-\sin^2t)}{(\frac{5}{2}\sin2t)^3}=\frac{3}{25\sin t\cos t}
\end{align*}
\begin{align*}
\tau(t)&=-\frac{x'''(z''y'-y''z')+y'''(x''z'-z''x')+z'''(y''x'-x''y')}{(z''y'-y''z')^2+(x''z'-z''x')^2+(y''x'-x''y')^2}\\
&=-\frac{\frac{9}{2}\sin^32t}{[15\sin^2t(1-\sin^2t)]^2}=-\frac{4}{25\sin t\cos t}
\end{align*}

\section{}
$$k(t)=\frac{x'y''-y'x''}{\sqrt{x'^2+y'^2}^3}=\frac{\cosh t}{\sqrt{1+\sinh^2t}^3}=\frac{1}{\cosh^2t}$$

\section{}
Let $t(s)$ be the unit tangent vector and $n(s)$ be the unit normal vector, from definition we know $t'(s)=k(s)n(s)=\dfrac{d\alpha/dt}{ds/dt}$, then
$$\alpha'=\frac{ds}{dt}t(s)$$
Differentiate both sides by $t$ and substitute $t'(s)$ by $k(s)n(s)$
$$\alpha''=\frac{d^2s}{dt^2}t(s)+\frac{ds}{dt}t'(s)=\frac{d^2s}{dt^2}t(s)+\frac{ds}{dt}k(s)n(s)$$
Multiple both sides by $t(s)$ as vector product
$$t(s)\land\alpha''=\frac{d^2s}{dt^2}[t(s)\land t(s)]+\frac{ds}{dt}k(s)[t(s)\land n(s)]$$
Taking norms of both sides
$$\left|\frac{d\alpha}{dt}\frac{dt}{ds}\land\alpha''\right|=0+\left|\left(\frac{ds}{dt}\right)^2k(t)\right|$$
Therefore
$$k(t)=\frac{|\alpha'\land\alpha''|}{|\alpha'|^3}$$



\section{}
$$k(t)=\frac{x'y''-y'x''}{\sqrt{x'^2+y'^2}^3}=\frac{ab\sin^2t+ab\cos^2t}{\sqrt{a^2\sin^2t+b^2\cos^2t}^3}=ab(a^2\sin^2t+b^2\cos^2t)^{-3/2}$$
$$k'(t)=ab(2a^2\sin t\cos t-2b^2\sin t\cos t)\cdot-\frac{3}{2}(a^2\sin^2t+b^2\cos^2t)^{-5/2}=0$$

Since it is an ellipse, we know that $ab\neq0,a^2-b^2\neq0$, and
$$a^2\sin^2t+b^2\cos^2t>\min\{a^2,b^2\}>0$$

So $$\sin t\cos t=0$$
$$t=2k\pi,\frac{(4k+1)\pi}{2},(2k+1)\pi,\frac{(4k+3)\pi}{2}\quad k\in Z$$

There are exactly four vertices, they are at $(a,0)$, $(0,b)$, $(-a,0)$ and $(0,-b)$.

\section{}

\end{document}
