\documentclass{article}
\usepackage{enumerate}
\usepackage{amsmath}
\usepackage{amssymb}
\usepackage{graphicx}
\usepackage{subfigure}
\usepackage{geometry}
\usepackage{caption}
\usepackage{indentfirst}
\geometry{left=3.0cm,right=3.0cm,top=3.0cm,bottom=4.0cm}
\usepackage{ctex}
\renewcommand\thesection{Ex \arabic{section}.}
\DeclareMathOperator*{\suplim}{\overline{\lim}}
\DeclareMathOperator*{\inflim}{\underline{\lim}}

\title{MA426 DIFFERENTIAL GEOMETRY HOMEWORK 2}
\author{刘逸灏 515370910207}
\date{\today}

\begin{document}
\maketitle

\section{}
$$r=(x,y,z)=(x,y,f(x,y))$$
$$r_x=(1,0,f_x(x,y))$$
$$r_y=(0,1,f_y(x,y))$$
$$r_x\land r_y=(-f_x,-f_y,1)$$
$$|r_x\land r_y|=\sqrt{1+f_x^2+f_y^2}$$
$$A=\iint_\Omega|r_x\land r_y|dxdy=\iint_\Omega\sqrt{1+f_x^2+f_y^2}dxdy$$

\section{}
For any constant $v$, the length curve $(u_1,u_2)\to R^3$ given by $X(u,v)$ is equal, let the length be $k_v$, then
$$\int_{u_1}^{u_2}\sqrt{E(u,v)}du=k_v$$

Take partial difference of $v$ on both sides, we can get
$$\int_{u_1}^{u_2}\frac{\partial\sqrt{E(u,v)}}{\partial v}du=0$$

Since $$\frac{\partial\sqrt{E(u,v)}}{\partial v}\geqslant0$$
$$\frac{\partial E}{\partial v}=0$$

For any constant $u$, the length curve $(v_1,v_2)\to R^3$ given by $X(u,v)$ is also equal, similarly, we can get
$$\frac{\partial G}{\partial u}=0$$

\section{}
$$r=(x,y,z)=(x,y,x^3)$$
$$r_x=(1,0,3x^2),r_y=(0,1,0)$$
$$E=r_x\cdot r_x=1+9x^4,F=r_x\cdot r_y=0,G=r_y\cdot r_y=1$$
$$n=\frac{r_x\land r_y}{|r_x\land r_y|}=\frac{(-3x^2,0,1)}{\sqrt{1+9x^4}}$$
$$r_{xx}=0,0,6x,r_{xy}=(0,0,0),r_{yy}=(0,0,0)$$
$$L=r_{xx}\cdot n=\frac{6x}{\sqrt{1+9x^4}},M=r_{xy}\cdot n=0,N=r_{yy}\cdot n=0$$

The mean curvature is
$$H=\frac{LG-2MF+NE}{2(EG-F^2)}=\frac{L}{2E}=\frac{3x}{(1+9x^4)^{1.5}}$$

The Gauss curvature is
$$K=\frac{LN-M^2}{EG-F^2}=0$$

\section{}
$$r=(t,v,X)=(t,v,\alpha(t)+v\omega(t))$$
$$r_t=(1,0,\alpha'(t)+v\omega'(t)),r_v=(0,1,\omega(t))$$
$$E=r_t\cdot r_t=1+[\alpha'(t)+v\omega'(t)]^2,F=r_t\cdot r_v=\omega(t)[\alpha'(t)+v\omega'(t)],G=r_v\cdot r_v=1+\omega^2(t)$$
$$n=\frac{r_t\land r_v}{|r_t\land r_v|}=\frac{(-[\alpha'(t)+v\omega'(t)],-\omega(t),1)}{\sqrt{1+\omega^2(t)+[\alpha'(t)+v\omega'(t)]^2}}$$
$$r_{tt}=(0,0,\alpha''(t)+v\omega''(t)),r_{tv}=(0,0,\omega'(t)),r_{vv}=(0,0,0)$$
$$L=r_{tt}\cdot n=\frac{\alpha''(t)+v\omega''(t)}{\sqrt{1+\omega^2(t)+[\alpha'(t)+v\omega'(t)]^2}},M=r_{tv}\cdot n=\frac{\omega'(t)}{\sqrt{1+\omega^2(t)+[\alpha'(t)+v\omega'(t)]^2}},N=r_{vv}\cdot n=(0,0,0)$$

Let $$a=\alpha'(t)+v\omega'(t),b=\omega(t)$$

The Gauss curvature is
$$K=\frac{LN-M^2}{EG-F^2}=\frac{-M^2}{EG-F^2}=-\frac{[\omega'(t)]^2}{(1+a^2+b^2)[(1+a^2)(1+b^2)-a^2b^2]}=-\frac{[\omega'(t)]^2}{\{1+[\alpha'(t)+v\omega'(t)]^2+\omega^2(t)\}^2}$$

\section{}
Let $z=\phi(s)$,
$$r(x,y,z)=(\phi(s)\cos\theta,\phi(s)\sin\theta,\phi(s))$$

\end{document}
